fairness/fair_termination.v
@@ -77,23 +77,27 @@ Proof.
     destruct Hev as [Hev|Hev]; first by destruct mtr; done.
     destruct mtr; first done. injection Hev => ->.
     apply terminating_trace_cons.
+    Local Ltac solve_fair Hfair := intros; eapply fair_by_cons; eauto; apply Hfair.
     eapply IH =>//; eauto.
     + eapply ftm_trans' =>//. apply Htrdec.
       punfold Hval. inversion Hval; simplify_eq; simpl in *; simplify_eq; done.
     + punfold Hval. inversion Hval; simplify_eq.
       destruct H4; done.
+    + solve_fair Hfair. 
   - simpl in *. destruct mtr; first (exists 1; done).
     rewrite -> !pred_at_S in Hev.
     punfold Hval; inversion Hval as [|??? Htrans Hval']; simplify_eq.
     destruct Hval' as [Hval'|]; last done.
     destruct (decide (ℓ = Some (ftm_decreasing_role s))) as [-> | Hnoteq].
     + apply terminating_trace_cons. eapply IH=>//; eauto.
-      eapply ftm_trans' =>//; apply Htrdec. simpl. destruct Hval;done.
+      2: { solve_fair Hfair. }
+      eapply ftm_trans' =>//; apply Htrdec. simpl. destruct Hval; done.
     + destruct mtr as [|s' ℓ' mtr''] eqn:Heq; first by eexists 2.
       destruct (ftm_decr (trfirst mtr)) as (Hlive' & Htrdec').
       { exists ℓ', (trfirst mtr''). punfold Hval'; inversion Hval'; subst; done. }
       apply terminating_trace_cons. eapply IHn=>//; eauto.
       * etransitivity; eauto. eapply ftm_notinc =>//.
+      * solve_fair Hfair. 
       * simplify_eq. eapply Hlive'.
       * erewrite <- ftm_decreasing_role_preserved =>//.
       * intros s'' Htrans''. eapply ftm_decr; eauto.
